tl.v moved to Type

yalla/tl.v
@@ -5,15 +5,16 @@
 
 (** * Example of a concrete use of the yalla library: tensor logic *)
 
-Require Import RelationClasses.
+Require Import CRelationClasses.
 Require Import Arith.
 Require Import Omega.
-Require Import Morphisms.
+Require Import CMorphisms.
 
 Require Import Injective.
 Require Import Bool_more.
 Require Import List_more.
-Require Import genperm.
+Require Import List_Type_more.
+Require Import genperm_Type.
 
 
 (** ** 0. load the [ill] library *)
@@ -34,6 +35,7 @@ Inductive tformula : Set :=
 | tplus : tformula -> tformula -> tformula
 | toc : tformula -> tformula.
 
+(* TODO
 Inductive tsubform : tformula -> tformula -> Prop :=
 | tsub_id : forall A, tsubform A A
 | tsub_tens_l : forall A B C, tsubform A B -> tsubform A (ttens B C)
@@ -58,6 +60,7 @@ split.
 - intros l1 l2 l3.
   apply tsub_trans.
 Qed.
+*)
 
 (** ** 2. define embedding into [iformula] *)
 
@@ -104,14 +107,14 @@ Qed.
 
 Lemma tl2ill_map_ioc_inv : forall l1 l2,
   map ioc l1 = map tl2ill l2 ->
-    exists l2', l2 = map toc l2' /\ l1 = map tl2ill l2'.
+    { l2' | l2 = map toc l2' & l1 = map tl2ill l2' }.
 Proof with try assumption ; try reflexivity.
 induction l1 ; intros l2 Heq ;
   destruct l2 ; inversion Heq...
 - exists nil ; split...
 - apply IHl1 in H1.
   destruct t ; inversion H0.
-  destruct H1 as (l2' & Heq1 & H1) ; subst.
+  destruct H1 as [l2' Heq1 H1] ; subst.
   exists (t :: l2') ; split...
 Qed.
 
@@ -120,13 +123,15 @@ Qed.
 
 Record tpfrag := mk_tpfrag {
   tpcut : bool ;
-  tpgax : list tformula -> option tformula -> Prop ;
+  tpgax : { tptypgax : Type & tptypgax -> list tformula * option tformula } ; (* Many thanks to Damien Pous! *)
   tpperm : bool }.
 
 Definition le_tpfrag P Q :=
-     Bool.leb (tpcut P) (tpcut Q)
-  /\ (forall f a, tpgax P f a -> tpgax Q f a)
-  /\ Bool.leb (tpperm P) (tpperm Q).
+  prod 
+     (Bool.leb (tpcut P) (tpcut Q))
+  (prod
+     (forall a, { b | projT2 (tpgax P) a = projT2 (tpgax Q) b })
+     (Bool.leb (tpperm P) (tpperm Q))).
 
 Lemma le_tpfrag_trans : forall P Q R,
   le_tpfrag P Q -> le_tpfrag Q R -> le_tpfrag P R.
@@ -135,10 +140,10 @@ intros P Q R H1 H2.
 destruct H1 as (Hc1 & Ha1 & Hp1).
 destruct H2 as (Hc2 & Ha2 & Hp2).
 split ; [ | split ] ; try (eapply leb_trans ; eassumption).
-intros f a Hax.
-apply Ha2.
-apply Ha1.
-assumption.
+intros a.
+destruct (Ha1 a) as [b Heq].
+destruct (Ha2 b) as [c Heq2].
+exists c ; etransitivity ; eassumption.
 Qed.
 
 Definition cutupd_tpfrag P b := mk_tpfrag b (tpgax P) (tpperm P).
@@ -147,9 +152,9 @@ Definition axupd_tpfrag P G := mk_tpfrag (tpcut P) G (tpperm P).
 
 Definition cutrm_tpfrag P := cutupd_tpfrag P false.
 
-Inductive tl P : list tformula -> option tformula -> Prop :=
+Inductive tl P : list tformula -> option tformula -> Type :=
 | ax_tr : forall X, tl P (tvar X :: nil) (Some (tvar X))
-| ex_tr : forall l1 l2 A, tl P l1 A -> PEperm (tpperm P) l1 l2 ->
+| ex_tr : forall l1 l2 A, tl P l1 A -> PEperm_Type (tpperm P) l1 l2 ->
                           tl P l2 A
 | one_trr : tl P nil (Some tone)
 | one_tlr : forall l1 l2 A, tl P (l1 ++ l2) A ->
@@ -189,10 +194,11 @@ Inductive tl P : list tformula -> option tformula -> Prop :=
 | cut_tr {f : tpcut P = true} : forall A l0 l1 l2 C,
                                tl P l0 (Some A) -> tl P (l1 ++ A :: l2) C ->
                                tl P (l1 ++ l0 ++ l2) C
-| gax_tr : forall l A, tpgax P l A -> tl P l A. 
+| gax_tr : forall a,
+           tl P (fst (projT2 (tpgax P) a)) (snd (projT2 (tpgax P) a)).
 
 Instance tl_perm {P} {Pi} :
-  Proper ((PEperm (tpperm P)) ==> Basics.impl) (fun l => tl P l Pi).
+  Proper ((PEperm_Type (tpperm P)) ==> Basics.arrow) (fun l => tl P l Pi).
 Proof.
 intros l1 l2 HP pi.
 eapply ex_tr ; eassumption.
@@ -204,27 +210,22 @@ intros Hle l A H.
 induction H ; try (constructor ; try assumption ; fail).
 - apply (ex_tr _ l1)...
   destruct Hle as (_ & _ & Hp).
-  hyps_PEperm_unfold ; unfold PEperm.
+  hyps_PEperm_Type_unfold ; unfold PEperm_Type.
   destruct (tpperm P) ; destruct (tpperm Q) ;
     simpl in Hp ; try inversion Hp ; subst...
 - destruct Hle as [Hcut _].
   rewrite f in Hcut.
   eapply (@cut_tr _ Hcut)...
-- apply gax_tr.
-  apply Hle...
-Qed.
-
-Instance Permutation_tl P Pi :
-  Proper ((PEperm (tpperm P)) ==> Basics.impl) (fun l => tl P l Pi).
-Proof.
-intros l1 l2 HP pi.
-eapply ex_tr ; eassumption.
+- destruct Hle as (_ & Hgax & _).
+  destruct (Hgax a) as [b Heq].
+  rewrite Heq.
+  apply gax_tr.
 Qed.
 
 
 (** ** 4. characterize corresponding [ill] fragment *)
 
-(*
+(* TODO
 Definition tl_fragment A := A = N \/ exists B, A = tl2ill B.
 
 Lemma tl_is_fragment : ifragment tl_fragment.
@@ -246,10 +247,12 @@ Qed.
 
 Definition t2ipfrag P := {|
   ipcut := tpcut P ;
-  ipgax := fun l C => 
-              (exists l0 C0, l = map tl2ill l0 /\ C = tl2ill C0 
-                        /\ tpgax P l0 (Some C0))
-           \/ (exists l0, l = map tl2ill l0 /\ C = N /\ tpgax P l0 None) ;
+  ipgax := existT (fun x => x -> list iformula * iformula) (projT1 (tpgax P))
+             (fun a => (map tl2ill (fst (projT2 (tpgax P) a)),
+                        match snd (projT2 (tpgax P) a) with
+                        | Some C => tl2ill C
+                        | None   => N
+                        end)) ;
   ipperm := tpperm P |}.
 
 Lemma cutrm_t2ipfrag : forall P,
@@ -262,8 +265,8 @@ Qed.
 (** ** 5. prove equivalence of proof predicates *)
 
 Lemma tl2tlfrag {P} : forall l C, tl P l C ->
-   (forall D, C = Some D -> exists s, ill (t2ipfrag P) (map tl2ill l) (tl2ill D) s)
-/\ (C = None -> exists s, ill (t2ipfrag P) (map tl2ill l) N s).
+   (forall D, C = Some D -> ill (t2ipfrag P) (map tl2ill l) (tl2ill D))
+ * (C = None -> ill (t2ipfrag P) (map tl2ill l) N).
 Proof with try eassumption ; try reflexivity.
 intros l C pi.
 induction pi ;
@@ -277,137 +280,53 @@ induction pi ;
   try rewrite ? map_app in piE1 ;
   try rewrite ? map_app in piS2 ;
   try rewrite ? map_app in piE2 ;
-  list_simpl.
+  list_simpl ;
+  (try now (constructor ; intuition)) ;
+  try now (destruct D ; inversion HeqC ; subst ; constructor ; intuition).
+- eapply ex_ir.
+  + apply (piS _ HeqC).
+  + apply PEperm_Type_map...
+- eapply ex_ir.
+  + apply (piE HeqC).
+  + apply PEperm_Type_map...
 - destruct D ; inversion HeqC ; subst.
-  eexists.
-  apply ax_ir.
-- destruct (piS _ HeqC) as [s0 pi0].
-  eexists.
-  eapply ex_ir... 
-  apply PEperm_map...
-- destruct (piE HeqC) as [s0 pi0].
-  eexists.
-  eapply ex_ir... 
-  apply PEperm_map...
-- destruct D ; inversion HeqC ; subst.
-  eexists.
-  apply one_irr.
-- destruct (piS _ HeqC) as [s0 pi0].
-  eexists.
-  apply one_ilr...
-- destruct (piE HeqC) as [s0 pi0].
-  eexists.
-  apply one_ilr...
-- destruct (piS1 _ (eq_refl _)) as [s1 pi1'].
-  destruct (piS2 _ (eq_refl _)) as [s2 pi2'].
-  destruct D ; inversion HeqC ; subst.
-  eexists.
-  eapply ex_ir.
-  + apply (tens_irr _ _ _ _ _ _ _ pi1' pi2').
-  + simpl ; PEperm_solve.
-- destruct (piS _ HeqC) as [s0 pi0].
-  eexists.
-  apply tens_ilr...
-- destruct (piE HeqC) as [s0 pi0].
-  eexists.
-  apply tens_ilr...
-- destruct D ; inversion HeqC ; subst.
-  destruct (piE (eq_refl _)) as [s0 pi0].
-  eexists.
-  apply neg_irr...
-- inversion HeqC.
-- destruct (piS _ (eq_refl _ )) as [s0 pi0].
-  eexists.
-  eapply ex_ir.
-  + eapply neg_ilr.
-    apply pi0.
-  + simpl ; PEperm_solve.
-- eexists.
-  apply zero_ilr.
-- eexists.
-  apply zero_ilr.
-- destruct (piS _ (eq_refl _)) as [s0 pi0].
-  destruct D ; inversion HeqC ; subst.
-  eexists.
-  apply plus_irr1...
-- destruct (piS _ (eq_refl _)) as [s0 pi0].
-  destruct D ; inversion HeqC ; subst.
-  eexists.
-  apply plus_irr2...
-- destruct (piS1 _ HeqC) as [s1 pi1'].
-  destruct (piS2 _ HeqC) as [s2 pi2'].
-  eexists.
-  apply plus_ilr...
-- destruct (piE1 HeqC) as [s1 pi1'].
-  destruct (piE2 HeqC) as [s2 pi2'].
-  eexists.
-  apply plus_ilr...
-- destruct (piS _ (eq_refl _)) as [s0 pi0].
-  destruct D ; inversion HeqC ; subst.
-  eexists.
   rewrite tl2ill_map_ioc ; simpl.
   apply oc_irr.
-  rewrite <- tl2ill_map_ioc...
-- destruct (piS _ HeqC) as [s0 pi0].
-  eexists.
-  apply de_ilr...
-- destruct (piE HeqC) as [s0 pi0].
-  eexists.
-  apply de_ilr...
-- destruct (piS _ HeqC) as [s0 pi0].
-  eexists.
-  apply wk_ilr...
-- destruct (piE HeqC) as [s0 pi0].
-  eexists.
-  apply wk_ilr...
-- destruct (piS _ HeqC) as [s0 pi0].
-  eexists.
-  list_simpl in pi0.
-  rewrite tl2ill_map_ioc.
+  rewrite <- tl2ill_map_ioc ; intuition.
+- rewrite tl2ill_map_ioc.
   simpl ; apply co_ilr.
-  rewrite <- tl2ill_map_ioc...
-- destruct (piE HeqC) as [s0 pi0].
-  eexists.
-  list_simpl in pi0.
-  rewrite tl2ill_map_ioc.
+  rewrite <- tl2ill_map_ioc.
+  assert (pi' := piS _ HeqC).
+  list_simpl in pi'...
+- rewrite tl2ill_map_ioc.
   simpl ; apply co_ilr.
-  rewrite <- tl2ill_map_ioc...
-- destruct (piS1 _ (eq_refl _ )) as [s1 pi1'].
-  destruct (piS2 _ HeqC) as [s2 pi2'].
-  eexists.
-  eapply ex_ir.
-  + eapply (cut_ir _ _ _ _ _ _ _ _ pi1' pi2').
-  + simpl ; PEperm_solve.
-- destruct (piS1 _ (eq_refl _ )) as [s1 pi1'].
-  destruct (piE2 HeqC) as [s2 pi2'].
-  eexists.
-  eapply ex_ir.
-  + eapply (cut_ir _ _ _ _ _ _ _ _ pi1' pi2').
-  + simpl ; PEperm_solve.
-- subst.
-  eexists.
-  apply gax_ir.
-  left.
-  eexists ; eexists ; split ; [ | split ]...
-- subst.
-  eexists.
-  apply gax_ir.
-  right.
-  eexists ; split ; [ | split ]...
+  rewrite <- tl2ill_map_ioc.
+  assert (pi' := piE HeqC).
+  list_simpl in pi'...
+- eapply ex_ir...
+  eapply (cut_ir _ _ _ _ _ _ (piS1 _ eq_refl) (piS2 _ HeqC))...
+- eapply ex_ir...
+  eapply (cut_ir _ _ _ _ _ _ (piS1 _ eq_refl) (piE2 HeqC))...
+- assert (pi := gax_ir (t2ipfrag P) a).
+  simpl in pi.
+  rewrite HeqC in pi...
+- assert (pi := gax_ir (t2ipfrag P) a).
+  simpl in pi.
+  rewrite HeqC in pi...
 Unshelve. all : simpl...
 Qed.
 
-Lemma tlfrag2tl_0 {P} : tpcut P = false -> forall l A s,
-  ill (t2ipfrag P) l A s ->
+Lemma tlfrag2tl_0 {P} : tpcut P = false -> forall l A,
+  ill (t2ipfrag P) l A ->
       (forall l0 A0, l = map tl2ill l0 -> A = tl2ill A0 -> tl P l0 (Some A0))
-  /\  (forall l0, l = map tl2ill l0 -> A = N -> tl P l0 None).
+    * (forall l0, l = map tl2ill l0 -> A = N -> tl P l0 None).
 Proof with try reflexivity ; try eassumption ; try omega.
 intros Hcut.
-intros l A s pi.
+intros l A pi.
 induction pi ;
   (split ; [ intros l'' A'' Heql HeqA | intros l'' Heql HeqN ]) ; subst ; 
   try (now (destruct A'' ; inversion HeqA)) ;
-  try (now (decomp_map Heql ; destruct x ; inversion Heql3)) ;
+  try (now (decomp_map_Type Heql ; destruct x ; inversion Heql3)) ;
   try (now inversion HeqN).
 - destruct l'' ; inversion Heql ;
     destruct l'' ; inversion Heql.
@@ -419,40 +338,38 @@ induction pi ;
   rewrite HeqN in Heql.
   destruct l'' ; inversion Heql.
   destruct t ; inversion H0.
-- apply PEperm_map_inv in H.
-  destruct H as (l0 & Heq & HP) ; subst.
+- apply PEperm_Type_map_inv in p.
+  destruct p as [l0 Heq HP] ; subst.
   eapply ex_tr.
   + apply IHpi...
-  + rewrite HP...
-- apply PEperm_map_inv in H.
-  destruct H as (l0 & Heq & HP) ; subst.
+  + symmetry...
+- apply PEperm_Type_map_inv in p.
+  destruct p as [l0 Heq HP] ; subst.
   symmetry in HP.
-  eapply ex_tr.
-  + apply IHpi...
-  + rewrite HP...
+  eapply ex_tr ; [ apply IHpi | ]...
 - destruct l'' ; inversion Heql.
   destruct A'' ; inversion HeqA ; subst.
   apply one_trr.
-- decomp_map Heql ; subst.
+- decomp_map_Type Heql ; subst.
   destruct x ; inversion Heql3 ; subst.
   apply one_tlr.
   apply IHpi...
   list_simpl...
-- decomp_map Heql ; subst.
+- decomp_map_Type Heql ; subst.
   destruct x ; inversion Heql3 ; subst.
   apply one_tlr.
   apply IHpi...
   list_simpl...
-- decomp_map Heql ; destruct A'' ; inversion HeqA ; subst.
+- decomp_map_Type Heql ; destruct A'' ; inversion HeqA ; subst.
   apply tens_trr.
   + apply IHpi1...
   + apply IHpi2...
-- decomp_map Heql ; subst.
+- decomp_map_Type Heql ; subst.
   destruct x ; inversion Heql3 ; subst.
   apply tens_tlr.
   apply IHpi...
   list_simpl...
-- decomp_map Heql ; subst.
+- decomp_map_Type Heql ; subst.
   destruct x ; inversion Heql3 ; subst.
   apply tens_tlr.
   apply IHpi...
@@ -460,15 +377,15 @@ induction pi ;
 - destruct A'' ; inversion HeqA ; subst.
   apply neg_trr.
   apply IHpi...
-- decomp_map Heql ; subst.
+- decomp_map_Type Heql ; subst.
   destruct x ; inversion Heql3 ; subst.
   destruct l3 ; inversion Heql4.
   apply neg_tlr.
   apply IHpi...
-- decomp_map Heql ; subst.
+- decomp_map_Type Heql ; subst.
   destruct x ; inversion Heql3 ; subst.
   apply zero_tlr.
-- decomp_map Heql ; subst.
+- decomp_map_Type Heql ; subst.
   destruct x ; inversion Heql3 ; subst.
   apply zero_tlr.
 - destruct A'' ; inversion HeqA ; subst.
@@ -477,14 +394,14 @@ induction pi ;
 - destruct A'' ; inversion HeqA ; subst.
   apply plus_trr2.
   apply IHpi...
-- decomp_map Heql ; subst.
+- decomp_map_Type Heql ; subst.
   destruct x ; inversion Heql3 ; subst.
   apply plus_tlr.
   + apply IHpi1...
     list_simpl...
   + apply IHpi2...
     list_simpl...
-- decomp_map Heql ; subst.
+- decomp_map_Type Heql ; subst.
   destruct x ; inversion Heql3 ; subst.
   apply plus_tlr.
   + apply IHpi1...
@@ -492,42 +409,42 @@ induction pi ;
   + apply IHpi2...
     list_simpl...
 - apply tl2ill_map_ioc_inv in Heql.
-  destruct Heql as (l0' & Heq & Heq') ; subst.
+  destruct Heql as [l0' Heq Heq'] ; subst.
   destruct A'' ; inversion HeqA ; subst.
   apply oc_trr.
   apply IHpi...
   rewrite tl2ill_map_ioc...
-- decomp_map Heql ; subst.
+- decomp_map_Type Heql ; subst.
   destruct x ; inversion Heql3 ; subst.
   apply de_tlr.
   apply IHpi...
   list_simpl...
-- decomp_map Heql ; subst.
+- decomp_map_Type Heql ; subst.
   destruct x ; inversion Heql3 ; subst.
   apply de_tlr.
   apply IHpi...
   list_simpl...
-- decomp_map Heql ; subst.
+- decomp_map_Type Heql ; subst.
   destruct x ; inversion Heql3 ; subst.
   apply wk_tlr.
   apply IHpi...
   list_simpl...
-- decomp_map Heql ; subst.
+- decomp_map_Type Heql ; subst.
   destruct x ; inversion Heql3 ; subst.
   apply wk_tlr.
   apply IHpi...
   list_simpl...
-- decomp_map Heql ; subst.
+- decomp_map_Type Heql ; subst.
   apply tl2ill_map_ioc_inv in Heql3.
-  destruct Heql3 as (l0' & Heq & Heq') ; subst.
+  destruct Heql3 as [l0' Heq Heq'] ; simpl in Heq ; subst.
   destruct x ; inversion Heql2 ; subst.
   apply co_tlr.
   apply IHpi...
   rewrite <- tl2ill_map_ioc.
   list_simpl...
-- decomp_map Heql ; subst.
+- decomp_map_Type Heql ; subst.
   apply tl2ill_map_ioc_inv in Heql3.
-  destruct Heql3 as (l0' & Heq & Heq') ; subst.
+  destruct Heql3 as [l0' Heq Heq'] ; simpl in Heq ; subst.
   destruct x ; inversion Heql2 ; subst.
   apply co_tlr.
   apply IHpi...
@@ -537,66 +454,62 @@ induction pi ;
   rewrite H0 in Hcut ; inversion Hcut.
 - inversion f.
   rewrite H0 in Hcut ; inversion Hcut.
-- destruct H as [ (l & C & Heq1 & Heq2 & Hax) | (l & Heq1 & Heq2 & Hax) ].
-  + apply tl2ill_inj in Heq2.
-    apply map_inj in Heq1 ; [ | apply tl2ill_inj ] ; subst.
-    apply gax_tr...
-  + exfalso.
-    destruct A'' ; inversion Heq2.
-- destruct H as [ (l & C & Heq1 & Heq2 & Hax) | (l & Heq1 & Heq2 & Hax) ].
-  + exfalso.
-    destruct C ; inversion Heq2.
-  + apply map_inj in Heq1 ; [ | apply tl2ill_inj ] ; subst.
-    apply gax_tr...
+- simpl in Heql ; simpl in HeqA.
+  case_eq (snd (projT2 (tpgax P) a)).
+  + intros A Heq.
+    rewrite_all Heq.
+    apply tl2ill_inj in HeqA ; subst.
+    rewrite <- Heq.
+    apply map_inj in Heql ; [ | apply tl2ill_inj ] ; subst.
+    apply gax_tr.
+  + intros Heq ; exfalso.
+    rewrite_all Heq.
+    destruct A'' ; inversion HeqA.
+- simpl in Heql ; simpl in HeqN.
+  case_eq (snd (projT2 (tpgax P) a)).
+  + intros A Heq ; exfalso.
+    rewrite_all Heq.
+    destruct A ; inversion HeqN.
+  + intros Heq.
+    rewrite_all Heq.
+    rewrite <- Heq.
+    apply map_inj in Heql ; [ | apply tl2ill_inj ] ; subst.
+    apply gax_tr.
 Qed.
 
-Lemma tlfrag2tl_cutfree {P} : tpcut P = false -> forall l s,
-   (forall A, ill (t2ipfrag P) (map tl2ill l) (tl2ill A) s -> tl P l (Some A))
-/\ (ill (t2ipfrag P) (map tl2ill l) N s -> tl P l None).
+Lemma tlfrag2tl_cutfree {P} : tpcut P = false -> forall l,
+   (forall A, ill (t2ipfrag P) (map tl2ill l) (tl2ill A) -> tl P l (Some A))
+ * (ill (t2ipfrag P) (map tl2ill l) N -> tl P l None).
 Proof with try reflexivity ; try assumption.
-intros l s ; split ; [ intros A | ] ; intros pi ; eapply tlfrag2tl_0 in pi...
+intros l ; split ; [ intros A | ] ; intros pi ; eapply tlfrag2tl_0 in pi...
 all : apply pi...
 Qed.
 
-Lemma tlfrag2tl_axfree {P} : (forall l C, ~ tpgax P l C) -> forall l s,
-   (forall A, ill (t2ipfrag P) (map tl2ill l) (tl2ill A) s -> tl P l (Some A))
-/\ (ill (t2ipfrag P) (map tl2ill l) N s -> tl P l None).
+Lemma tlfrag2tl_axfree {P} : (forall a : projT1 (tpgax P), False) -> forall l,
+   (forall A, ill (t2ipfrag P) (map tl2ill l) (tl2ill A) -> tl P l (Some A))
+ * (ill (t2ipfrag P) (map tl2ill l) N -> tl P l None).
 Proof with try reflexivity ; try assumption.
 intros Hgax.
-intros l s ; split ; [ intros A | ] ; intros pi.
+intros l ; split ; [ intros A | ] ; intros pi.
 - apply (cut_admissible_ill_nzeropos_axfree_by_ll _ i2ac_inj) in pi...
-  + clear s ; destruct pi as [s pi].
-    rewrite cutrm_t2ipfrag in pi.
+  + rewrite cutrm_t2ipfrag in pi.
     apply tlfrag2tl_cutfree in pi...
     apply (stronger_tpfrag (cutrm_tpfrag P))...
-    split ; [ | split ]...
-    intros f a Hax...
-  + intros l' C' Hax.
-    destruct Hax as [(l'' & C'' & Hl & HC & Hax) | (l'' & Hl & HC & Hax)] ;
-      apply Hgax in Hax...
+    split ; [ | split ] ; intuition...
   + replace (tl2ill A :: map tl2ill l)
       with (map tl2ill (A :: l)) by (list_simpl ; reflexivity).
-    apply Forall_forall.
-    intros x Hin.
-    apply in_map_iff in Hin.
-    destruct Hin as (x0 & Heq & _) ; subst.
+    remember (A :: l) as l0 ; clear.
+    induction l0 ; simpl ; constructor ; intuition.
     apply tl2ill_nz.
 - apply (cut_admissible_ill_nzeropos_axfree_by_ll _ i2ac_inj) in pi...
-  + clear s ; destruct pi as [s pi].
-    rewrite cutrm_t2ipfrag in pi.
+  + rewrite cutrm_t2ipfrag in pi.
     apply tlfrag2tl_cutfree in pi...
     apply (stronger_tpfrag (cutrm_tpfrag P))...
-    split ; [ | split ]...
-    intros f a Hax...
-  + intros l' C' Hax.
-    destruct Hax as [(l'' & C'' & Hl & HC & Hax) | (l'' & Hl & HC & Hax)] ;
-      apply Hgax in Hax...
-  + constructor ; [ constructor | ]...
-    apply Forall_forall.
-    intros x Hin.
-    apply in_map_iff in Hin.
-    destruct Hin as (x0 & Heq & _) ; subst.
-    apply tl2ill_nz.
+    split ; [ | split ] ; intuition...
+  + constructor.
+    * constructor.
+    * clear ; induction l ; simpl ; constructor ; intuition.
+      apply tl2ill_nz.
 Qed.
 
 
@@ -607,86 +520,66 @@ Qed.
 Lemma ax_gen_r {P} : forall A, tl P (A :: nil) (Some A).
 Proof.
 intro A.
-destruct (@ax_exp_ill (t2ipfrag (cutrm_tpfrag P)) (tl2ill A))
-  as [s Hax].
 apply (stronger_tpfrag (cutrm_tpfrag P)).
 - split ; [ | split ] ; simpl ; try reflexivity.
-  intros f a Has ; assumption.
+  intros a ; exists a ; reflexivity.
 - eapply tlfrag2tl_cutfree ; try reflexivity.
-  eassumption.
+  apply ax_exp_ill.
 Qed.
 
 (** *** cut elimination *)
 
-Lemma cut_tl_r_axfree {P} : (forall l C, ~ tpgax P l C) -> forall A l0 l1 l2 C,
+Lemma cut_tl_r_axfree {P} : (forall a : projT1 (tpgax P), False) -> forall A l0 l1 l2 C,
   tl P l0 (Some A) -> tl P (l1 ++ A :: l2) C -> tl P (l1 ++ l0 ++ l2) C.
 Proof with try reflexivity ; try eassumption.
 intros Hgax.
 intros A l0 l1 l2 C pi1 pi2.
 destruct (tl2tlfrag _ _ pi1) as [pi1' _] ; simpl in pi1'.
-destruct (pi1' _ (eq_refl _)) as [s1 pi1''].
+assert (pi1'' := pi1' _ eq_refl).
 destruct (tl2tlfrag _ _ pi2) as [pi2' pi2''].
 case_eq (tpcut P) ; intros Hcut.
 - eapply cut_tr...
 - case_eq C.
   + intros D HeqD.
-    destruct (pi2' _ HeqD) as [s pi].
+    assert (pi := pi2' _ HeqD).
     list_simpl in pi.
     eapply (cut_ir_nzeropos_axfree_by_ll _ i2ac_inj _ _ _ (map tl2ill l1)
-                                                 (map tl2ill l2) _ _ _ _ pi1'')
+                                                 (map tl2ill l2) _ _ pi1'')
       in pi...
-    clear s ; destruct pi as [s pi].
     rewrite <- ? map_app in pi.
     apply tlfrag2tl_cutfree in pi...
   + intros HeqD.
-    destruct (pi2'' HeqD) as [s pi].
+    assert (pi := pi2'' HeqD).
     list_simpl in pi.
     eapply (cut_ir_nzeropos_axfree_by_ll _ i2ac_inj _ _ _ (map tl2ill l1)
-                                                 (map tl2ill l2) _ _ _ _ pi1'')
+                                                 (map tl2ill l2) _ _ pi1'')
       in pi...
-    clear s ; destruct pi as [s pi].
     rewrite <- ? map_app in pi.
     apply tlfrag2tl_cutfree in pi...
 Unshelve.
-* intros l C0 Hax ; inversion Hax.
-  -- destruct H as (l' & C' & Hl & HC & H).
-     apply Hgax in H...
-  -- destruct H as (l' & Hl & HC & H).
-     apply Hgax in H...
+all : try intuition.
 * replace (tl2ill D :: map tl2ill l1 ++ map tl2ill l0 ++ map tl2ill l2)
      with (map tl2ill (D :: l1 ++ l0 ++ l2)) by (list_simpl ; reflexivity).
-  apply Forall_forall.
-  intros x Hin.
-  apply in_map_iff in Hin.
-  destruct Hin as (x0 & Heq & _) ; subst.
+  remember (D :: l1 ++ l0 ++ l2) as l ; clear.
+  induction l ; simpl ; constructor ; intuition.
   apply tl2ill_nz.
-* intros l C0 Hax ; inversion Hax.
-  -- destruct H as (l' & C' & Hl & HC & H).
-     apply Hgax in H...
-  -- destruct H as (l' & Hl & HC & H).
-     apply Hgax in H...
-* constructor ; [ constructor | ].
-  replace (map tl2ill l1 ++ map tl2ill l0 ++ map tl2ill l2)
-     with (map tl2ill (l1 ++ l0 ++ l2)) by (list_simpl ; reflexivity).
-  apply Forall_forall.
-  intros x Hin.
-  apply in_map_iff in Hin.
-  destruct Hin as (x0 & Heq & _) ; subst.
-  apply tl2ill_nz.
+* constructor.
+  -- constructor.
+  -- rewrite <- ? map_app.
+     remember (l1 ++ l0 ++ l2) as l ; clear.
+     induction l ; simpl ; constructor ; intuition.
+     apply tl2ill_nz.
 Qed.
 
-Lemma cut_admissible_tl_axfree {P} : (forall l C, ~ tpgax P l C) ->
+Lemma cut_admissible_tl_axfree {P} : (forall a : projT1 (tpgax P), False) ->
   forall l Pi, tl P l Pi -> tl (cutrm_tpfrag P) l Pi.
 Proof with try reflexivity ; try eassumption.
 intros Hgax.
 intros l Pi pi.
-induction pi ;
-  try (constructor ; eassumption ; fail) ;
-  try (destruct IHpi as [s' IHpi] ; constructor ; eassumption ; fail) ;
-  try (destruct IHpi1 as [s'1 IHpi1] ;
-       destruct IHpi2 as [s'2 IHpi2] ; constructor ; eassumption ; fail).
+induction pi ; try now constructor.
 - apply (ex_tr _ l1)...
 - eapply cut_tl_r_axfree...
+- intuition.
 Qed.
 
 (** *** conservativity with respect to [ll] *)
@@ -742,56 +635,41 @@ Unshelve.
 Qed.
 *)
 
-Theorem ll_is_tl_axfree {P} : (forall l C, ~ tpgax P l C) -> forall l,
-  (forall A, tl P l (Some A)
-         <-> exists s,
-             ll (i2pfrag i2ac (t2ipfrag P)) (ill2ll i2ac (tl2ill A) ::
-                          rev (map dual (map (ill2ll i2ac) (map tl2ill l)))) s)
-/\          (tl P l None
-         <-> exists s,
-             ll (i2pfrag i2ac (t2ipfrag P)) (ill2ll i2ac N ::
-                          rev (map dual (map (ill2ll i2ac) (map tl2ill l)))) s).
+Theorem ll_is_tl_axfree {P} : (forall a : projT1 (tpgax P), False) -> forall l,
+   (forall A, tl P l (Some A)
+           -> ll (i2pfrag i2ac (t2ipfrag P)) (ill2ll i2ac (tl2ill A) ::
+                           rev (map dual (map (ill2ll i2ac) (map tl2ill l)))))
+ * (forall A, ll (i2pfrag i2ac (t2ipfrag P)) (ill2ll i2ac (tl2ill A) ::
+                           rev (map dual (map (ill2ll i2ac) (map tl2ill l))))
+           -> tl P l (Some A))
+ *           (tl P l None
+           -> ll (i2pfrag i2ac (t2ipfrag P)) (ill2ll i2ac N ::
+                           rev (map dual (map (ill2ll i2ac) (map tl2ill l)))))
+ *           (ll (i2pfrag i2ac (t2ipfrag P)) (ill2ll i2ac N ::
+                          rev (map dual (map (ill2ll i2ac) (map tl2ill l))))
+           -> tl P l None).
 Proof with try eassumption.
-intros Hgax.
-split ; split ; intros pi ; try destruct pi as [s pi].
+intros Hgax l.
+split ; [ split ; [ split | ] | ] ; (try intros A pi) ; try intros pi.
 - apply tl2tlfrag in pi.
-  destruct (proj1 pi _ (eq_refl _)) as [s pi'].
-  eapply ill_to_ll...
+  eapply ill_to_ll ; intuition.
 - eapply (ll_to_ill_nzeropos_axfree _ i2ac_inj _ (ill2ll i2ac (tl2ill A)
             :: rev (map dual (map (ill2ll i2ac) (map tl2ill l))))) in pi ;
     [ | | reflexivity ]...
-  + clear s ; destruct pi as [s pi].
-    apply tlfrag2tl_axfree in pi...
+  + apply tlfrag2tl_axfree...
   + change (tl2ill A :: map tl2ill l) with (map tl2ill (A :: l)).
-    apply Forall_forall.
-    intros x Hin.
-    apply in_map_iff in Hin.
-    destruct Hin as (s0 & Heq & Hin) ; subst.
+    remember (A :: l) as l0 ; clear.
+    induction l0 ; simpl ; constructor ; intuition.
     apply tl2ill_nz.
 - apply tl2tlfrag in pi.
-  destruct (proj2 pi (eq_refl _)) as [s pi'].
-  eapply ill_to_ll...
+  eapply ill_to_ll ; intuition.
 - eapply (ll_to_ill_nzeropos_axfree _ i2ac_inj _ (ill2ll i2ac N
             :: rev (map dual (map (ill2ll i2ac) (map tl2ill l))))) in pi ;
     [ | | reflexivity ]...
-  + clear s ; destruct pi as [s pi].
-    apply tlfrag2tl_axfree in pi...
+  + apply tlfrag2tl_axfree...
   + constructor ; [ constructor | ].
-    apply Forall_forall.
-    intros x Hin.
-    apply in_map_iff in Hin.
-    destruct Hin as (s0 & Heq & Hin) ; subst.
+    clear ; induction l ; simpl ; constructor ; intuition.
     apply tl2ill_nz.
-Unshelve.
-* intros l0 C0 Hax ; inversion Hax.
-  -- destruct H as (l' & C' & Hl & HC & H).
-     apply Hgax in H...
-  -- destruct H as (l' & Hl & HC & H).
-     apply Hgax in H...
-* intros l0 C0 Hax ; inversion Hax.
-  -- destruct H as (l' & C' & Hl & HC & H).
-     apply Hgax in H...
-  -- destruct H as (l' & Hl & HC & H).
-     apply Hgax in H...
+Unshelve. all : intuition.
 Qed.
 
